Update AllocVar lemma for space cost
There are two cheats:

 - we need an invariant that connects dataSem's limits to the
   actual heap limit

 - the statement that size_of soundly (over)approximates
   the size of the live data after a GC run is cheated

Development from here can go both outwards, i.e. propagate
this space information to other theorem statemets, and
inwards, i.e. prove the cheats mentioned above.

Currently, AllocVar only makes a statement about space usage
if the Simple GC is used. The same should in the future be
proved for the Generational GC. These proofs are not going to
cover the case gc_kind = None.

compiler/backend/proofs/data_to_word_gcProofScript.sml
@@ -4189,6 +4189,25 @@ val abs_ml_inv_ADD = prove(
   fs [abs_ml_inv_def,gc_kind_inv_def] \\ rw []
   \\ fs [gen_state_ok_def]);
 
+val alloc_size_def = Define `
+  alloc_size k = (if k * (dimindex (:'a) DIV 8) < dimword (:α) then
+                    n2w (k * (dimindex (:'a) DIV 8))
+                  else (-1w)):'a word`
+
+Theorem alloc_size_check:
+  w2n (bytes_in_word * n2w k2 :'a word) < w2n (alloc_size k :'a word) ==>
+  k2 * (dimindex (:α) DIV 8) < dimword (:α) /\ good_dimindex (:'a) ==>
+  k2 < k
+Proof
+  rw [alloc_size_def,bytes_in_word_def]
+  \\ fs [word_mul_n2w]
+  \\ fs [NOT_LESS]
+  \\ qsuff_tac `0 < dimindex (:α) DIV 8 /\ k2 < k` THEN1 fs []
+  \\ rewrite_tac [GSYM LT_MULT_RCANCEL]
+  \\ match_mp_tac LESS_LESS_EQ_TRANS
+  \\ qexists_tac `dimword (:'a)` \\ fs []
+QED
+
 Theorem word_gc_fun_correct:
    good_dimindex (:'a) /\
     heap_in_memory_store heap a sp sp1 gens c s m dm limit /\
@@ -4197,7 +4216,10 @@ Theorem word_gc_fun_correct:
       word_gc_fun c (MAP SND stack,m,dm,s) = SOME (stack1,m1,s1) /\
       heap_in_memory_store heap1 a1 sp1 sp2 gens2 c s1 m1 dm limit /\
       word_ml_inv (heap1,be,a1,sp1,sp2,gens2) limit ts c refs
-        ((v,s1 ' Globals)::ZIP (MAP FST stack,stack1))
+        ((v,s1 ' Globals)::ZIP (MAP FST stack,stack1)) /\
+      (has_space (Word ((alloc_size k):'a word)) (t with store := s1) = SOME F /\
+       c.gc_kind = Simple ==>
+         sp1 + sp2 < k)
 Proof
   full_simp_tac(srw_ss())[word_ml_inv_def]
   \\ srw_tac[][] \\ drule (GEN_ALL gc_combined_thm)
@@ -4212,10 +4234,19 @@ Proof
   \\ drule (GEN_ALL word_gc_fun_lemma |> ONCE_REWRITE_RULE [CONJ_COMM]
              |> REWRITE_RULE [GSYM CONJ_ASSOC]) \\ fs []
   \\ rpt (disch_then drule) \\ strip_tac \\ fs [] \\ rfs []
+  \\ fs [PULL_EXISTS]
   \\ rveq \\ Cases_on `c.gc_kind` \\ fs []
   \\ rpt (asm_exists_tac \\ fs [MAP_ZIP] \\ rfs [MAP_ZIP])
   \\ imp_res_tac abs_ml_inv_ADD
   \\ rpt (asm_exists_tac \\ fs [MAP_ZIP] \\ rfs [MAP_ZIP])
+  \\ fs [heap_in_memory_store_def]
+  \\ fs [abs_ml_inv_def,unused_space_inv_def,wordSemTheory.has_space_def]
+  \\ fs [WORD_LEFT_ADD_DISTRIB,GSYM word_add_n2w]
+  \\ fs [GSYM NOT_LESS] \\ rw []
+  \\ drule alloc_size_check
+  \\ disch_then match_mp_tac \\ fs []
+  \\ fs [heap_ok_def] \\ rveq \\ fs [good_dimindex_def]
+  \\ rfs [dimword_def]
 QED
 
 
@@ -5418,11 +5449,6 @@ Proof
   \\ full_simp_tac(srw_ss())[LENGTH_LASTN_LESS]
 QED
 
-val alloc_size_def = Define `
-  alloc_size k = (if k * (dimindex (:'a) DIV 8) < dimword (:α) then
-                    n2w (k * (dimindex (:'a) DIV 8))
-                  else (-1w)):'a word`
-
 Theorem NOT_1_domain:
    ~(1 IN domain (adjust_set names))
 Proof
@@ -6155,6 +6181,9 @@ Theorem state_rel_gc:
       dec_stack wl t.stack = SOME stack /\
       FLOOKUP st (Temp 29w) = FLOOKUP t.store (Temp 29w) /\
       FLOOKUP st AllocSize = SOME (Word (alloc_size k)) /\
+      (has_space (Word ((alloc_size k):'a word)) (t with <|store := st |>) = SOME F /\
+       c.gc_kind = Simple ==>
+         s.limits.heap_limit < size_of_heap s + k) /\
       state_rel c l1 l2 (s with space := 0)
         (t with <|stack := stack; store := st; memory := m|>) [] locs
 Proof
@@ -6184,6 +6213,18 @@ Proof
          \\ rpt (pairarg_tac \\ fs []) \\ rveq
          \\ every_case_tac \\ fs [] \\ rveq
          \\ fs [FLOOKUP_UPDATE,FUPDATE_LIST] \\ EVAL_TAC)
+  \\ conj_tac
+  THEN1
+   (Cases_on `c.gc_kind = Simple` \\ fs []
+    \\ fs [wordSemTheory.has_space_def] \\ strip_tac \\ fs []
+    \\ fs [option_case_eq,CaseEq"word_loc"] \\ rveq \\ fs []
+    \\ `s.limits.heap_limit = limit` by cheat (* make it an inv *)
+    \\ pop_assum (fn th => fs [th])
+    \\ `sp1 + sp2 <= limit` by
+     (fs [word_ml_inv_def,abs_ml_inv_def,heap_ok_def] \\ rveq \\ fs []
+      \\ fs [unused_space_inv_def])
+    \\ qsuff_tac `limit - (sp1 + sp2) <= size_of_heap s` THEN1 fs []
+    \\ cheat (* this is the interesting proof *))
   \\ fs [code_oracle_rel_def,FLOOKUP_UPDATE]
   \\ imp_res_tac stack_rel_dec_stack_IMP_stack_rel \\ full_simp_tac(srw_ss())[]
   \\ asm_exists_tac \\ full_simp_tac(srw_ss())[]
@@ -6203,6 +6244,21 @@ Proof
   \\ fs [word_simpProofTheory.is_gc_word_const_def,isWord_def]
 QED
 
+Definition cut_locals_def:
+  cut_locals names s =
+    case cut_env names s.locals of
+    | SOME env => s with locals := env
+    | NONE => s with locals := LN
+End
+
+Theorem size_of_heap_call_push_env:
+  cut_env names s.locals = SOME x ==>
+  size_of_heap (call_env [] (push_env x F s)) = size_of_heap (s with locals := x)
+Proof
+  fs [push_env_def,call_env_def,size_of_heap_def,stack_to_vs_def,
+      extract_stack_def,EVAL ``toList (fromList []:'a spt)``]
+QED
+
 Theorem gc_lemma:
    let t0 = call_env [Loc l1 l2] (push_env y
         (NONE:(num # 'a wordLang$prog # num # num) option) t) in
@@ -6217,6 +6273,8 @@ Theorem gc_lemma:
         pop_env (t0 with <|stack := stack; store := st; memory := m|>) = SOME t2 /\
         FLOOKUP t2.store (Temp 29w) = FLOOKUP t.store (Temp 29w) ∧
         FLOOKUP t2.store AllocSize = SOME (Word (alloc_size k)) /\
+        (has_space (Word ((alloc_size k):'a word)) t2 = SOME F /\ c.gc_kind = Simple ==>
+           s.limits.heap_limit < size_of_heap (s with locals := x) + k) /\
         state_rel c l1 l2 (s with <| locals := x; space := 0 |>) t2 [] locs
 Proof
   srw_tac[][] \\ full_simp_tac(srw_ss())[LET_DEF]
@@ -6248,6 +6306,10 @@ Proof
   \\ Cases_on `env_to_list y t.permute` \\ full_simp_tac(srw_ss())[LET_DEF]
   \\ every_case_tac \\ full_simp_tac(srw_ss())[]
   \\ srw_tac[][] \\ full_simp_tac(srw_ss())[]
+  \\ fs [wordSemTheory.has_space_def]
+  \\ drule size_of_heap_call_push_env \\ strip_tac \\ fs []
+  \\ `(call_env [] (push_env x F s)).limits.heap_limit = s.limits.heap_limit`
+        by fs [call_env_def,push_env_def] \\ fs []
 QED
 
 Theorem gc_add_call_env:
@@ -6358,7 +6420,10 @@ Theorem alloc_lemma:
     alloc (alloc_size k) (adjust_set names)
         (t with locals := insert 1 (Word (alloc_size k)) t.locals) =
       ((q:'a result option),r) ==>
-    (q = SOME NotEnoughSpace ⇒ r.ffi = s.ffi) ∧
+    (q = SOME NotEnoughSpace ⇒
+     r.ffi = s.ffi /\
+     (c.gc_kind = Simple ==>
+       s.limits.heap_limit < size_of_heap (cut_locals names s) + k)) ∧
     (q ≠ SOME NotEnoughSpace ⇒
      state_rel c l1 l2 (s with <|locals := x; space := k|>) r [] locs ∧
      alloc_size k <> -1w:'a word /\
@@ -6403,6 +6468,7 @@ Proof
   \\ imp_res_tac wordPropsTheory.pop_env_const \\ full_simp_tac(srw_ss())[]
   \\ UNABBREV_ALL_TAC
   \\ full_simp_tac(srw_ss())[wordSemTheory.set_store_def,state_rel_def]
+  \\ fs [cut_locals_def]
   \\ qpat_assum `has_space (Word (alloc_size k)) r = SOME T` assume_tac
   \\ CCONTR_TAC \\ fs [wordSemTheory.has_space_def]
   \\ rfs [heap_in_memory_store_def,FLOOKUP_DEF,FAPPLY_FUPDATE_THM]
@@ -6464,10 +6530,21 @@ Proof
   fs [alloc_size_def,EVAL ``good_dimindex (:'a)``] \\ rw [] \\ fs []
 QED
 
-val alloc_fail = alloc_lemma
+val alloc_fail_lemma = alloc_lemma
   |> Q.INST [`k`|->`dimword (:'a)`]
   |> SIMP_RULE std_ss [UNDISCH alloc_size_dimword]
   |> DISCH_ALL |> MP_CANON
+  |> SIMP_RULE std_ss [AC ADD_COMM ADD_ASSOC]
+
+Theorem alloc_fail:
+  good_dimindex (:α) ∧ state_rel c l1 l2 ^s t [] locs ∧
+  cut_env names s.locals = SOME x ∧
+  alloc (-1w:'a word) (adjust_set names)
+    (t with locals := insert 1 (Word (-1w)) t.locals) = (q,r) ⇒
+  (q = SOME NotEnoughSpace ⇒ r.ffi = s.ffi) ∧ q = SOME NotEnoughSpace
+Proof
+  metis_tac [alloc_fail_lemma]
+QED
 
 val word_exp_rw = save_thm("word_exp_rw",LIST_CONJ
   [wordSemTheory.word_exp_def,
@@ -6562,7 +6639,9 @@ Theorem AllocVar_thm:
     get_var 1 t = SOME (Word w) /\
     evaluate (AllocVar c limit names,t) = (q,r) /\
     limit < dimword (:'a) DIV 8 ==>
-    (q = SOME NotEnoughSpace ⇒ r.ffi = s.ffi) ∧
+    (q = SOME NotEnoughSpace ⇒ r.ffi = s.ffi ∧
+          (c.gc_kind = Simple /\ w2n w DIV 4 < limit ⇒
+           s.limits.heap_limit < size_of_heap (cut_locals names s) + w2n w DIV 4 + 1)) ∧
     (q ≠ SOME NotEnoughSpace ⇒
       w2n w DIV 4 < limit /\
       state_rel c l1 l2 (s with <|locals := x; space := w2n w DIV 4 + 1|>) r [] locs ∧
@@ -6694,7 +6773,6 @@ Proof
           |> SIMP_RULE std_ss [AND_IMP_INTRO] |> GEN_ALL)
     \\ qexists_tac `t1` \\ fs [Abbr`t1`]
     \\ fs [state_rel_insert_3]
-    \\ asm_exists_tac \\ fs []
     \\ qpat_assum `_ = (q,r)` (fn th => fs [GSYM th])
     \\ simp [insert_insert_3_1]
     \\ pairarg_tac \\ fs []
@@ -6719,7 +6797,7 @@ Proof
     \\ strip_tac \\ Cases_on `n=1` \\ fs []
     \\ Cases_on `n=3` \\ fs []
     \\ rw [] \\ drule domain_adjust_set_EVEN \\ EVAL_TAC)
-  \\ fs []
+  \\ fs [cut_locals_def]
   \\ match_mp_tac (alloc_alt |> SPEC_ALL
         |> Q.INST [`s`|->`s with locals := z`]
         |> SIMP_RULE (srw_ss()) []
@@ -6729,7 +6807,7 @@ Proof
         |> DISCH ``(t:('a,'c,'ffi) wordSem$state).data_buffer = c2``
         |> DISCH ``(t:('a,'c,'ffi) wordSem$state).compile = c3``
         |> DISCH ``(t:('a,'c,'ffi) wordSem$state).compile_oracle = c4``
-        |> SIMP_RULE std_ss [AND_IMP_INTRO] |> GEN_ALL) \\ fs []
+        |> SIMP_RULE (srw_ss()) [AND_IMP_INTRO,cut_locals_def] |> GEN_ALL) \\ fs []
   \\ qexists_tac `x`
   \\ qexists_tac `t with locals := y` \\ fs []
   \\ simp [GSYM PULL_EXISTS]
@@ -7029,6 +7107,5 @@ val word_ml_inv_get_var_IMP = save_thm("word_ml_inv_get_var_IMP",
   |> Q.INST [`n`|->`[n1]`,`x`|->`[x1]`] |> GEN_ALL
   |> REWRITE_RULE [get_vars_SOME_IFF,get_vars_SOME_IFF_data,MAP]
   |> SIMP_RULE std_ss [Once get_vars_sing,PULL_EXISTS,get_vars_SOME_IFF,ZIP,APPEND]);
-
 
 val _ = export_theory();
